@prefix g36: <http://data.ashrae.org/standard223/1.0/extensions/g36#> .
@prefix owl: <http://www.w3.org/2002/07/owl#> .
@prefix quantitykind: <http://qudt.org/vocab/quantitykind/> .
@prefix qudt: <http://qudt.org/schema/qudt/> .
@prefix rdf: <http://www.w3.org/1999/02/22-rdf-syntax-ns#> .
@prefix rdfs: <http://www.w3.org/2000/01/rdf-schema#> .
@prefix s223: <http://data.ashrae.org/standard223#> .
@prefix sh: <http://www.w3.org/ns/shacl#> .
@prefix xsd: <http://www.w3.org/2001/XMLSchema#> .

g36:SingleZoneVAVAirHandlingUnit a s223:Class,
        rdfs:Class,
        sh:NodeShape ;
    rdfs:label "SingleZoneVAVAirHandlingUnit" ;
    rdfs:comment "An assembly consisting of sections containing a fan or fans and other necessary equipment to perform one or more of the following functions: circulating, filtration, heating, cooling, heat recovery, humidifying, dehumidifying, and mixing of air. It is usually connected to an air-distribution system. This air handling unit that serves one zone only." ;
    rdfs:subClassOf s223:AirHandlingUnit ;
    sh:property [ rdfs:comment "The SingleZoneVAVAirHandlingUnit shall contain at least one supply fan with a VFD that has the role Supply using the relation contains." ;
            sh:message "g36: The SingleZoneVAVAirHandlingUnit shall contain at least one supply fan with a VFD that has the role Supply using the relation contains." ;
            sh:minCount 1 ;
            sh:path s223:contains ;
            sh:qualifiedMinCount 1 ;
            sh:qualifiedValueShape [ sh:class g36:FanWithVFD ;
                    sh:node [ sh:property [ sh:hasValue s223:Role-Supply ;
                                    sh:path s223:hasRole ] ] ] ;
             ],
        [ rdfs:comment "A SingleZoneVAVAirHandlingUnit OutletConnectionPoint shall have at least one supply air temperature property using the relation hasProperty." ;
            sh:message "g36: A SingleZoneVAVAirHandlingUnit OutletConnectionPoint shall have at least one supply air temperature property using the relation hasProperty." ;
            sh:minCount 1 ;
            sh:path s223:hasConnectionPoint ;
            sh:qualifiedMinCount 1 ;
            sh:qualifiedValueShape [ sh:class s223:OutletConnectionPoint ;
                    sh:node [ sh:property [ sh:minCount 1 ;
                                    sh:path s223:hasProperty ;
                                    sh:qualifiedMinCount 1 ;
                                    sh:qualifiedValueShape [ sh:class s223:QuantifiableObservableProperty ;
                                            sh:node [ sh:property [ sh:hasValue quantitykind:Temperature ;
                                                            sh:maxCount 1 ;
                                                            sh:minCount 1 ;
                                                            sh:path qudt:hasQuantityKind ],
                                                        [ sh:hasValue s223:Role-Supply ;
                                                            sh:maxCount 1 ;
                                                            sh:minCount 1 ;
                                                            sh:path s223:hasAspect ] ] ] ] ] ] ;
             ],
        [ rdfs:comment "The SingleZoneVAVAirHandlingUnit shall have at least one outdoor air damper using the relation contains." ;
            sh:message "g36: The SingleZoneVAVAirHandlingUnit shall have at least one outdoor air damper using the relation contains." ;
            sh:minCount 1 ;
            sh:path s223:contains ;
            sh:qualifiedMinCount 1 ;
            sh:qualifiedValueShape [ sh:class g36:Damper ;
                    sh:node [ sh:property [ sh:minCount 1 ;
                                    sh:path s223:hasRole ;
                                    sh:qualifiedMinCount 1 ;
                                    sh:qualifiedValueShape [ sh:hasValue s223:Role-OutdoorAirIntake ] ] ] ] ;
             ],
        [ rdfs:comment "The SingleZoneVAVAirHandlingUnit shall have at least one return air damper using the relation contains." ;
            sh:message "g36: The SingleZoneVAVAirHandlingUnit shall have at least one return air damper using the relation contains." ;
            sh:minCount 1 ;
            sh:path s223:contains ;
            sh:qualifiedMinCount 1 ;
            sh:qualifiedValueShape [ sh:class g36:Damper ;
                    sh:node [ sh:property [ sh:minCount 1 ;
                                    sh:path s223:hasRole ;
                                    sh:qualifiedMinCount 1 ;
                                    sh:qualifiedValueShape [ sh:hasValue s223:Role-Return ] ] ] ] ;
             ],
        [ rdfs:comment "The  SingleZoneVAVAirHandlingUnit shall contain at least one ChilledWaterCoil for cooling using the relation contains." ;
            sh:message "g36: The  SingleZoneVAVAirHandlingUnit shall contain at least one ChilledWaterCoil for cooling using the relation contains." ;
            sh:minCount 1 ;
            sh:path s223:contains ;
            sh:qualifiedMinCount 1 ;
            sh:qualifiedValueShape [ sh:class g36:ChilledWaterCoil ] ;
             ],
        [ rdfs:comment "The SingleZoneVAVAirHandlingUnit shall contain at least one HotWaterCoil or at least one ElectricHeatingCoil for heating using the relation contains." ;
            sh:message "g36: The SingleZoneVAVAirHandlingUnit shall contain at least one HotWaterCoil or at least one ElectricHeatingCoil for heating using the relation contains." ;
            sh:minCount 1 ;
            sh:path s223:contains ;
            sh:qualifiedMinCount 1 ;
            sh:qualifiedValueShape [ sh:or ( [ sh:class g36:HotWaterCoil ] [ sh:class g36:ElectricHeatingCoil ] ) ] ;
             ] ;
     .

g36:SingleZoneVAVAirHandlingUnit-WithReliefDamper a s223:Class,
        rdfs:Class,
        sh:NodeShape ;
    rdfs:comment "A SingleZoneVAVAirHandlingUnit with a relief air damper and no relief fan" ;
    rdfs:label "Single Zone VAV Air Handling Unit With Relief Damper" ;
    rdfs:subClassOf g36:SingleZoneVAVAirHandlingUnit ;
    sh:class s223:AirHandlingUnit ;
    sh:property [ rdfs:comment "the SingleZoneVAVAirHandlingUnit contains a relief air damper with a modulating actuator." ;
            sh:path s223:contains ;
            sh:qualifiedMinCount 1 ;
            sh:qualifiedValueShape [ sh:class g36:Damper ;
                    sh:node [ sh:property [ sh:hasValue s223:Role-Relief ;
                                    sh:maxCount 1 ;
                                    sh:minCount 1 ;
                                    sh:path s223:hasRole ],
                                [ sh:minCount 1 ;
                                    sh:path s223:hasProperty ;
                                    sh:qualifiedMinCount 1 ;
                                    sh:qualifiedValueShape [ sh:class s223:QuantifiableActuatableProperty ;
                                            sh:node [ sh:property [ sh:hasValue quantitykind:DimensionlessRatio ;
                                                            sh:maxCount 1 ;
                                                            sh:minCount 1 ;
                                                            sh:path qudt:hasQuantityKind ],
                                                        [ sh:hasValue s223:Binary-Position ;
                                                            sh:maxCount 1 ;
                                                            sh:minCount 1 ;
                                                            sh:path s223:hasAspect ] ] ] ] ] ] ;
             ] .

g36:SingleZoneVAVAirHandlingUnit-WithReliefFan a s223:Class,
        rdfs:Class,
        sh:NodeShape ;
    rdfs:comment "A SingleZoneVAVAirHandlingUnit with a relief fan and relief dampers" ;
    rdfs:label "Single Zone VAV Air Handling Unit With Relief Fan" ;
    rdfs:subClassOf g36:SingleZoneVAVAirHandlingUnit ;
    sh:class s223:AirHandlingUnit ;
    sh:property [ rdfs:comment "For the case where the SingleZoneVAVAirHandlingUnit has both a relief air damper and a relief fan, the SingleZoneVAVAirHandlingUnit must indeed have a relief air damper with a two-position damper command property." ;
            sh:path s223:contains ;
            sh:qualifiedMaxCount 1 ;
            sh:qualifiedMinCount 1 ;
            sh:qualifiedValueShape [ sh:class g36:TwoPositionDamper ;
                    sh:node [ sh:property [ sh:path s223:hasRole ;
                                    sh:qualifiedMinCount 1 ;
                                    sh:qualifiedValueShape [ sh:hasValue s223:Role-Relief ] ] ] ] ;
             ],
        [ rdfs:comment "For the case where the SingleZoneVAVAirHandlingUnit has both a relief air damper and a relief fan, the SingleZoneVAVAirHandlingUnit must indeed have a relief fan." ;
            sh:path s223:contains ;
            sh:qualifiedMaxCount 1 ;
            sh:qualifiedMinCount 1 ;
            sh:qualifiedValueShape [ sh:class g36:FanWithVFD ;
                    sh:node [ sh:property [ sh:path s223:hasRole ;
                                    sh:qualifiedMinCount 1 ;
                                    sh:qualifiedValueShape [ sh:hasValue s223:Role-Relief ] ] ] ] ;
             ],
        [ rdfs:comment "For the case where the SingleZoneVAVAirHandlingUnit has both a relief air damper and a relief fan, the SingleZoneVAVAirHandlingUnit must be connectedTo at least one VAV, which is connectedTo at least one HVAC DomainSpace or Zone, which has a building static pressure property." ;
            sh:path ( [ sh:oneOrMorePath s223:connectedTo ] sh:zeroOrOnePath [ sh:inversePath s223:hasDomainSpace ] ) ;
            sh:qualifiedMinCount 1 ;
            sh:qualifiedValueShape [ sh:node [ sh:property [ sh:hasValue s223:Domain-HVAC ;
                                    sh:maxCount 1 ;
                                    sh:minCount 1 ;
                                    sh:path s223:hasDomain ],
                                [ sh:path s223:hasProperty ;
                                    sh:qualifiedMinCount 1 ;
                                    sh:qualifiedValueShape [ sh:class s223:QuantifiableObservableProperty ;
                                            sh:node [ sh:property [ sh:hasValue quantitykind:Pressure ;
                                                            sh:maxCount 1 ;
                                                            sh:minCount 1 ;
                                                            sh:path qudt:hasQuantityKind ] ] ] ] ] ] ;
             ] .

g36:SingleZoneVAVAirHandlingUnit-WithReturnFan a s223:Class,
        rdfs:Class,
        sh:NodeShape ;
    rdfs:comment "A SingleZoneVAVAirHandlingUnit with a Return fan" ;
    rdfs:label "Single Zone VAV Air Handling Unit With Return Fan" ;
    rdfs:subClassOf g36:SingleZoneVAVAirHandlingUnit ;
    sh:class s223:AirHandlingUnit ;
    sh:property [ rdfs:comment "For the case where the SingleZoneVAVAirHandlingUnit has a return fan, the SingleZoneVAVAirHandlingUnit must indeed contain a return fan." ;
            sh:path s223:contains ;
            sh:qualifiedMinCount 1 ;
            sh:qualifiedValueShape [ sh:class g36:FanWithVFD ;
                    sh:node [ sh:property [ sh:hasValue s223:Role-Return ;
                                    sh:minCount 1 ;
                                    sh:path s223:hasRole ] ] ] ;
             ],
        [ rdfs:comment "For the case where the SingleZoneVAVAirHandlingUnit has a return fan, the SingleZoneVAVAirHandlingUnit must contain an exhaust air damper with either an analog or two-position damper command property." ;
            sh:path s223:contains ;
            sh:qualifiedMinCount 1 ;
            sh:qualifiedValueShape [ sh:node [ sh:property [ sh:hasValue s223:Role-Exhaust ;
                                    sh:maxCount 1 ;
                                    sh:minCount 1 ;
                                    sh:path s223:hasRole ] ] ;
                    sh:or ( [ sh:class g36:Damper ] [ sh:class g36:TwoPositionDamper ] ) ] ;
             ] .

g36:SingleZoneVAVAirHandlingUnit-WithReliefFanAnnotation a sh:NodeShape ;
    sh:rule [ a sh:TripleRule ;
            rdfs:comment "If an instance of s223:AirHandlingUnit matches the constraints defined by g36:SingleZoneVAVAirHandlingUnit and has a relief fan, it will be declared as an instance of this class." ;
            sh:condition [ sh:property [ sh:path s223:contains ;
                            sh:qualifiedMaxCount 1 ;
                            sh:qualifiedMinCount 1 ;
                            sh:qualifiedValueShape [ sh:class g36:FanWithVFD ;
                                    sh:node [ sh:property [ sh:path s223:hasRole ;
                                                    sh:qualifiedMinCount 1 ;
                                                    sh:qualifiedValueShape [ sh:hasValue s223:Role-Relief ] ] ] ] ;
                             ]], g36:SingleZoneVAVAirHandlingUnit ;
            sh:object g36:SingleZoneVAVAirHandlingUnit-WithReliefFan ;
            sh:predicate rdf:type ;
            sh:subject sh:this ] ;
    sh:targetClass s223:AirHandlingUnit .

g36:SingleZoneVAVAirHandlingUnit-WithReturnFanAnnotation a sh:NodeShape ;
    sh:rule [ a sh:TripleRule ;
            rdfs:comment "If an instance of s223:AirHandlingUnit matches the constraints defined by g36:SingleZoneVAVAirHandlingUnit and has a return fan, it will be declared as an instance of that class." ;
            sh:condition [ sh:property [ rdfs:comment "For the case where the SingleZoneVAVAirHandlingUnit has both a Return air damper and a Return fan, the SingleZoneVAVAirHandlingUnit must indeed have a Return fan." ;
                            sh:path s223:contains ;
                            sh:qualifiedMaxCount 1 ;
                            sh:qualifiedMinCount 1 ;
                            sh:qualifiedValueShape [ sh:class g36:FanWithVFD ;
                                    sh:node [ sh:property [ sh:path s223:hasRole ;
                                                    sh:qualifiedMinCount 1 ;
                                                    sh:qualifiedValueShape [ sh:hasValue s223:Role-Return ] ] ] ] ;
                             ]],g36:SingleZoneVAVAirHandlingUnit ;
            sh:object g36:SingleZoneVAVAirHandlingUnit-WithReturnFan ;
            sh:predicate rdf:type ;
            sh:subject sh:this ] ;
    sh:targetClass s223:AirHandlingUnit .

g36:SingleZoneVAVAirHandlingUnitAnnotation a sh:NodeShape ;
    sh:rule [ a sh:TripleRule ;
            rdfs:comment "If an instance of s223:AirHandlingUnit matches the constraints defined by g36:SingleZoneVAVAirHandlingUnit, it will be declared as an instance of that class." ;
            sh:condition g36:SingleZoneVAVAirHandlingUnit ;
            sh:object g36:SingleZoneVAVAirHandlingUnit ;
            sh:predicate rdf:type ;
            sh:subject sh:this ] ;
    sh:targetClass s223:AirHandlingUnit .

<http://data.ashrae.org/standard223/1.0/extensions/g36#g36:SingleZoneVAVAirHandlingUnit-WithReliefDamperAnnotation> a sh:NodeShape ;
    sh:rule [ a sh:TripleRule ;
            rdfs:comment "If an instance of s223:AirHandlingUnit matches the constraints defined by g36:SingleZoneVAVAirHandlingUnit-WithReliefDamperFan, it will be declared as an instance of that class." ;
            sh:condition g36:SingleZoneVAVAirHandlingUnit-WithReliefDamper ;
            sh:object g36:SingleZoneVAVAirHandlingUnit-WithReliefDamper ;
            sh:predicate rdf:type ;
            sh:subject sh:this ] ;
    sh:targetClass s223:AirHandlingUnit .

<http://data.ashrae.org/standard223/1.0/extensions/g36/singlezone-vav-air-handling-unit> a owl:Ontology ;
    owl:imports <http://data.ashrae.org/standard223/1.0/extensions/settings>,
        <http://data.ashrae.org/standard223/1.0/model/all> ;
    owl:versionInfo "Created with TopBraid Composer" .

